src/case_study/list_example.v
@@ -1,14 +1,14 @@
 From iris.base_logic Require Export gen_heap.
 From iris.algebra Require Export list excl_auth.
 From nextgen.case_study.program_logic Require Import CC_ectx_lifting
-     CC_ectxi_language CC_ectx_lifting weakestpre.
+     CC_ectxi_language CC_ectx_lifting weakestpre cl_weakestpre.
 From nextgen.case_study Require Export stack_lang stack_transform.
 From iris.proofmode Require Import tactics.
 From stdpp Require Import fin_maps.
 
 From nextgen Require Import nextgen_independent.
 From nextgen.lib Require Import invariants.
-From nextgen.case_study Require Import rules_unary stack_lang_notation.
+From nextgen.case_study Require Import rules_unary cl_rules_unary stack_lang_notation.
 
 Set Default Proof Using "Type".
 Import uPred.
@@ -21,7 +21,7 @@ Lemma fill_to_CC_fill K n e :
 Proof. auto. Qed.
 
 Ltac peel_ctx :=
-  try rewrite fill_to_CC_fill; rewrite fill_inner_cons; simpl fill_item.
+  try rewrite fill_to_CC_fill; try rewrite fill_inner_cons; simpl fill_item.
 
 Ltac prepare_ctx :=
   (try rewrite /stack_fill_item /=) ;
@@ -29,8 +29,13 @@ Ltac prepare_ctx :=
   match goal with
   | |- context [ WP (?n,?e) @ _ ; ↑ _ ; _ {{ _ }}%I ] =>
       pose proof (construct_ctx_eq n e) as H;try rewrite /= to_of_val in H;
+      try rewrite /= construct_ctx_of_val in H;
       try (rewrite H; clear H; simpl app); peel_ctx
-      end.
+  | |- context [ CLWP (?n,?e) @ ↑ _ ; _ {{ _ }}%I ] =>
+      pose proof (construct_ctx_eq n e) as H;try rewrite /= to_of_val in H;
+      try rewrite /= construct_ctx_of_val in H;
+      try (rewrite H; clear H; simpl app); peel_ctx
+  end.
 
 Section list_code.
   Open Scope val_scope.
@@ -46,21 +51,7 @@ Section list_code.
       | SOME "p" =>
           let: "hd" := Fst !"p" in
           let: "tl" := Snd !"p" in
-          heap_cons ("f" "hd") ("map_list" "tl")
-      end.
-
-  Definition stack_cons : val :=
-    λ: global, <>, "x" "xs" := let: "p" := ⟪"x","xs"⟫ in
-                               SOME (sref "p").
-
-  Definition stack_map_list : val :=
-    rec: global, <>, "map_list", "f" "l" :=
-      match: "l" with
-        NONE => NONE
-      | SOME "p" =>
-          let: "hd" := Fst !"p" in
-          let: "tl" := Snd !"p" in
-          stack_cons ("f" "hd") ("map_list" "tl")
+          heap_cons ("f" "hd") ("map_list" "f" "tl")
       end.
 
   Definition empty_list : val := NONEV.
@@ -76,12 +67,6 @@ Section list_prec.
     | x :: xs => ∃ l hd', ⌜hd = SOMEV #(global,l)⌝ ∗ l ↦ ⟪x,hd'⟫ ∗ is_heap_list_nat hd' xs
   end%I.
 
-  Fixpoint is_stack_list_nat (i : nat) (hd : val) (xs : list nat) : iProp Σ :=
-    match xs with
-    | [] => ⌜hd = NONEV⌝
-    | x :: xs => ∃ l hd' j, ⌜hd = SOMEV #(global,l)⌝ ∗ ⌜j <= i⌝ ∗ j @@ l ↦ ⟪x,hd'⟫ ∗ is_stack_list_nat i hd' xs
-  end%I.
-
   Lemma is_heap_list_nat_intro hd xs lft :
     is_heap_list_nat hd xs ⊢ ⚡={Ω <- lft}=> is_heap_list_nat hd xs.
   Proof.
@@ -92,6 +77,20 @@ Section list_prec.
       iDestruct (IHxs with "Hlist") as "Hlist".
       iModIntro. iExists _,_. iFrame. auto.
   Qed.
+
+  #[global] Instance is_heap_list_nat_intro' hd xs lft
+    : IntoPnextgen _ _ _ := is_heap_list_nat_intro hd xs lft.
+
+  Lemma is_heap_list_nat_ind_intro hd xs lft :
+    is_heap_list_nat hd xs ⊢ ⚡◻{ Ω ↑ lft } is_heap_list_nat hd xs.
+  Proof.
+    apply bnextgen_bounded_ind_GenIndependent_intro.
+    simpl. iIntros (c Hc) "HP".
+    rewrite -next_state_eq. iModIntro. auto.
+  Qed.
+
+  #[global] Instance is_heap_list_nat_ind_intro' hd xs c
+    : IntoInextgen Ω c _ _ := is_heap_list_nat_ind_intro hd xs c.
 
   Lemma is_heap_list_shift hd xs :
     is_heap_list_nat hd xs -∗ ⌜∀ n, shift_val hd n = Some hd⌝.
@@ -113,66 +112,122 @@ Section list_prec.
       iPureIntro. repeat constructor.
   Qed.
 
-  Lemma is_stack_list_nat_intro i hd xs j :
-    i < j ->
-    is_stack_list_nat i hd xs ⊢ ⚡={Ω <- ^j}=> is_stack_list_nat i hd xs.
-  Proof.
-    intros Hlt.
-    revert hd. induction xs=>hd.
-    - simpl. iIntros "%". iModIntro. auto.
-    - simpl.
-      iIntros "(%l & %hd' & %i' & %Heq & %Hle & Hl & Hlist)".
-      iDestruct (IHxs with "Hlist") as "Hlist".
-      iDestruct (stack_stack_pop_intro _ _ _ _ j with "Hl") as "Hl";[lia|].
-      iModIntro. iExists _,_,_. iFrame. auto.
-  Qed.
-
-  Lemma is_stack_list_nat_weaken i i' hd xs :
-    i <= i' ->
-    is_stack_list_nat i hd xs ⊢ is_stack_list_nat i' hd xs.
-  Proof.
-    revert hd. induction xs=>hd.
-    - simpl. auto.
-    - simpl.
-      iIntros (Hle) "(%l & %hd' & %j & %Heq & %Hj & Hl & Hlist)".
-      iDestruct (IHxs with "Hlist") as "Hlist";auto.
-      iExists _,_,_. iFrame. iSplit;auto.
-      iPureIntro. lia.
-  Qed.
-
-  #[global] Instance is_heap_list_nat_intro' hd xs lft
-    : IntoPnextgen _ _ _ := is_heap_list_nat_intro hd xs lft.
-  
 End list_prec.
 
 Section list_spec.
   Context `{!heapGS Σ Ω}.
-  
-  Lemma heap_list_cons_spec hd xs (n : nat) m :
-    {{{ [size] m ∗ is_heap_list_nat hd xs }}}
-      (m,heap_cons n hd) @ ↑^m
-    {{{ hd', RET hd'; [size] m ∗ is_heap_list_nat hd'.2 (n :: xs) }}}.
-  Proof.
-    iIntros (Φ) "[Hsize Hlist] #HΦ /=". prepare_ctx.
-    iApply wp_call_global;[eauto|iFrame]. iIntros "!> Hsize /=". prepare_ctx.
-    iApply wp_return;[replace (S m - 1) with m by lia;apply rc_l|auto|lia|iFrame].
-    iIntros "!> Hsize /=". replace (m - 0) with m by lia. iModIntro. rewrite /stack_fill_item /=.
-    eassert (fill [] _ = _) as <-;eauto.
-    iDestruct (is_heap_list_shift with "Hlist") as %Hshift.
-    iApply wp_call_global;[eauto|eauto|iFrame]. iIntros "!> Hsize /=". prepare_ctx.
-    iApply wp_LetIn;[|iIntros "!> /=";simpl subst'].
-    { instantiate (1:=(_,⟪#nv n,_⟫%V)). rewrite /IntoVal/=/stack_of_val. f_equal;eauto. }
-    prepare_ctx. iDestruct (is_heap_list_permanent with "Hlist") as %Hpermanent.
-    iApply wp_heap_alloc.
-    { instantiate (1:=⟪#nv n,_⟫%V). rewrite /IntoVal/=/stack_of_val. f_equal;eauto. }
-    { constructor;auto. constructor. }
-    iIntros "!> %l Hl /=". prepare_ctx.
-    iApply wp_return;[replace (S m - 1) with m by lia;apply rc_l|auto|lia|iFrame].
-    iIntros "!> Hsize". iModIntro. simpl. replace (m - 0) with m by lia.
-    iApply wp_value. simpl.
-    iApply "HΦ". iFrame. iExists l,hd.
-    simpl. iFrame. auto.
-  Qed.
 
+  (* TODO: need to repeat the instance declaration for some reason *)
+  #[global] Instance heap_stack_ind_intro' l q v n
+    : IntoInextgen _ _ _ _ := heap_stack_ind_intro' l q v n.
+
+  Notation "c1 ≤ c2" := (rc locality_lifetime_rel c1 c2) (at level 70).
+  
+  Lemma heap_list_cons_spec hd xs (n : nat) m c :
+    c ≤ (^m) ->
+    [size] m ∗ is_heap_list_nat hd xs -∗
+    CLWP (m,heap_cons n hd) @ ↑c {{ hd', [size] m ∗ is_heap_list_nat hd'.2 (n :: xs) }}.
+  Proof.
+    intros Hle.
+    assert (∀ lft, GenIndependent CR (λ c : C, build_trans (gT_map (transmap_insert_two_inG
+                       (inv_pick_transform c) (C_pick c) Ω))) lft (is_heap_list_nat hd xs)).
+    { intros lft. iIntros (c' Hc) "Hlist". rewrite -/(nextgen_omega _ _) -next_state_eq. by iModIntro. }
+    iIntros "[Hsize Hlist] /=". prepare_ctx. iApply clwp_bind.
+    iApply (clwp_call_global (λ v, ⌜v.2 = _⌝)%I);[auto|eauto|iFrame]. iSplitL;cycle 1.
+    { iNext. iIntros "Hsize/=". iApply clwp_value;simpl;eauto. }
+    iNext. iModIntro. iIntros (v) "[Hsize %Heq] /=". simpl in Heq. rewrite Heq.
+    rewrite /stack_fill_item /=. iDestruct (is_heap_list_shift with "Hlist") as %Hshift.
+    iApply (clwp_call_global (λ v, is_heap_list_nat v.2 (n :: xs))%I);
+      [rewrite /IntoVal/=/stack_of_val/=;eauto|auto|eauto|iFrame].
+    iDestruct (is_heap_list_permanent with "Hlist") as %Hperm.
+    iSplitR;cycle 1.
+    { iNext. iIntros "Hsize /=".
+      iApply clwp_LetIn;[instantiate (1:=(_,⟪#nv n,_⟫%V)); eauto|]. iIntros "!> /=". prepare_ctx.
+      iApply clwp_bind.
+      iApply clwp_heap_alloc;[instantiate (1:=⟪#nv n,_⟫%V);eauto|repeat constructor;auto|..].
+      iIntros "!> %l Hl /=".
+      iApply clwp_value. rewrite /stack_fill_item /=.
+      iApply clwp_value. simpl. iExists _. iFrame. do 2 (iSplit;[eauto|]).
+      iExists l,hd. iFrame. auto. }
+    iIntros "!> !> %v' (Hsize & Hlist) /=". iFrame.
+  Qed.
+  
+  Lemma heap_list_map_list_spec (φ : nat -> nat -> Prop) hd xs (f : val) m c :
+    c ≤ (^m) ->
+    (∀ n, shift_val f n = Some f) -> (* if f is a heap closure, shifting it yields no changes *)
+    (∀ x v, expr_subst x v f = f) -> (* f is a closed expression *)
+    (⚡◻{ Ω ↑ #∞ } □ ∀ m' c (n : nat), ⌜c ≤ ^m'⌝ -∗ [size] m' -∗ CLWP (m',f (#nv n)) @ ↑c {{ λ v, ∃ n', ⌜v = (m',#nv n')⌝ ∗ ⌜φ n n'⌝ ∗ [size] m' }}) (* ⚡◻{ Ω ↑ #∞ } because f is a heap closure *) -∗
+    [size] m -∗
+    is_heap_list_nat hd xs -∗
+    CLWP (m,heap_map_list f hd) @ ↑c {{ λ hd', ⌜hd'.1 = m⌝ ∗ [size] m ∗ ∃ l, is_heap_list_nat hd'.2 l ∗ ⌜Forall2 (λ n1 n2, φ n1 n2) xs l⌝ }}.
+  Proof.
+    intros Hle Hshift Hclosed.
+    revert m hd Hle. induction xs;intros m hd Hle;iIntros "#Hspec Hsize Hlist".
+    - iDestruct "Hlist" as %->. simpl. prepare_ctx.
+      iApply clwp_bind.
+      iApply (clwp_call_global (λ v, ⌜v.2 = _⌝)%I);[eauto|auto|eauto|iFrame]. iSplitL;cycle 1.
+      { iNext. iIntros "Hsize/=". iApply clwp_value;simpl;eauto. }
+      iIntros "/= !> !> %v [Hsize ->]". rewrite /stack_fill_item/=.
+      iApply (clwp_call_global (λ v, (∃ l, is_heap_list_nat v.2 l ∗ ⌜_ l⌝))%I);[auto|eauto|]. simpl. iFrame. iSplitR.
+      { iIntros "!>!> %v [Hsize [%l [Hlist %Hres]]]". iFrame. iSplit;auto. }
+      iIntros "!> Hsize /=".
+      iApply clwp_case_injl. iIntros "!>/=".
+      iApply clwp_value. iExists _. simpl. do 2 (iSplit;[eauto|]). iFrame.
+      iExists []. auto.
+    - simpl is_heap_list_nat.
+      iDestruct "Hlist" as "(%l & %hd' & -> & Hl & Hlist)". prepare_ctx.
+      iApply clwp_bind.
+      iApply (clwp_call_global (λ v, ⌜v.2 = _⌝)%I);[eauto|auto|eauto|iFrame]. iSplitL;cycle 1.
+      { iNext. iIntros "Hsize/=". iApply clwp_value;simpl;eauto. }
+      rewrite bnextgen_bounded_ind_weaken_once;[|instantiate (1:=c);repeat constructor].
+      iIntros "/= !> !> %v [Hsize ->]". rewrite /stack_fill_item/=.
+      iApply (clwp_call_global (λ v, (∃ l, is_heap_list_nat v.2 l ∗ ⌜_ l⌝))%I);[auto|eauto|]. simpl. iFrame. iSplitR.
+      { iIntros "!>!> %v [Hsize [%l' [Hlist %Hres]]]". iFrame. auto. }
+      iIntros "!> Hsize /=".
+      iApply clwp_case_injr. iIntros "!>/=". prepare_ctx.
+      iApply clwp_bind.
+      iApply clwp_heap_load;[constructor|]. iFrame. iIntros "!> Hl".
+      iApply clwp_value;[instantiate (1:=(_,⟪ #nv a, hd' ⟫%V));eauto|simpl]. prepare_ctx.
+      iApply clwp_bind. iApply clwp_fst;[eexists (_,_);eauto|]. iIntros "!>/=".
+      iApply clwp_value. rewrite /stack_fill_item/=.
+      iApply clwp_LetIn. iIntros "!>/=". prepare_ctx.
+      iApply clwp_bind.
+      iApply clwp_heap_load;[constructor|]. iFrame. iIntros "!> Hl".
+      iApply clwp_value;[instantiate (1:=(_,⟪ #nv a, hd' ⟫%V));eauto|simpl]. prepare_ctx.
+      iApply clwp_bind. iApply clwp_snd;[instantiate (1:=(_,_));eauto|]. iIntros "!>/=".
+      iApply clwp_value;[instantiate (1:=(_,_));eauto|]. rewrite /stack_fill_item/=.
+      iApply clwp_LetIn;[instantiate (1:=(_,_));eauto|]. iIntros "!>/=".
+      rewrite !Hclosed. prepare_ctx.
+      iApply clwp_bind.
+      assert (c ≤ (^S m)) as Hle';[etrans;eauto;do 2 constructor;lia|].
+      iApply (clwp_wand with "[Hsize]").      
+      { rewrite 2!bnextgen_bounded_ind_elim. iApply ("Hspec" with "[%] Hsize"). auto. }
+      iIntros "!> %n (%n' & -> & %Hn & Hsize) /=". rewrite /stack_of_val/stack_fill_item/=.
+      prepare_ctx. iApply clwp_bind. 
+      iApply (clwp_call_global (λ v, ⌜v.2 = _⌝)%I);[auto|eauto|iFrame]. iSplitL;cycle 1.
+      { iNext. iIntros "Hsize/=". iApply clwp_value;simpl;eauto. }
+      iIntros "/= !> !> %v [Hsize ->]".
+      (* inductive call *)
+      prepare_ctx. rewrite fill_inner_cons. simpl fill_item. rewrite -/(heap_map_list _ _).
+      iApply clwp_bind.
+      iApply (clwp_wand with "[Hsize Hlist]").
+      { rewrite bnextgen_bounded_ind_elim. iApply (IHxs with "[//] Hsize Hlist"). auto. }
+      iIntros "!> %v (%Heq & Hsize & %l' & Hlist & %Hspec) /=". destruct v;simpl in Heq;subst.
+      simpl. rewrite /stack_of_val/stack_fill_item/=.
+      iDestruct (is_heap_list_shift with "Hlist") as %Hshift'.
+      iDestruct (is_heap_list_permanent with "Hlist") as %Hperm'.
+      iApply (clwp_call_global (λ v, ⌜shift_val v.2 (-1) = Some v.2⌝ ∗ is_heap_list_nat v.2 (n' :: l'))%I);[eauto|auto|eauto|iFrame].
+      iSplitL "Hl";cycle 1.
+      { iIntros "!> Hsize". simpl.
+        iApply clwp_LetIn;[instantiate (1:=(_,⟪#nv n',_⟫%V)); eauto|]. iIntros "!> /=". prepare_ctx.
+        iApply clwp_bind.
+        iApply clwp_heap_alloc;[instantiate (1:=⟪#nv n',_⟫%V);eauto|repeat constructor;auto|..].
+        iIntros "!> %l2 Hl2 /=".
+        iApply clwp_value. rewrite /stack_fill_item /=.
+        iApply clwp_value. simpl. iExists _. iFrame. do 3 (iSplit;[eauto|]).
+        iExists l2,v. iFrame. auto. }
+      iIntros "!> !> %v' (Hsize & %Hshift2 & Hlist)". iExists _. iFrame. do 2 (iSplit;[eauto|]).
+      iExists (n' :: l'). iFrame. iPureIntro. apply Forall2_cons. split;auto.
+  Qed.
     
 End list_spec.
