src/case_study/program_logic/cl_weakestpre.v
@@ -5,7 +5,7 @@
 
 From nextgen.case_study.program_logic Require Export weakestpre.
 From nextgen.case_study.program_logic Require Import CC_ectx_language CC_ectxi_language CC_ectx_lifting.
-
+From nextgen Require Import nextgen_independent.
 From iris.proofmode Require Import tactics.
 Set Default Proof Using "Type".
 Import uPred.
@@ -15,7 +15,7 @@ Section clwp_def.
   Context `{irisGS_gen hlc (CC_ectx_lang expr) Σ Ω T}.
 
 Definition clwp_def (c : C) (E : coPset) (e : expr) (Φ : val → iProp Σ) : iProp Σ :=
-  (∀ K Ψ, (∀ v, Φ v -∗ WP fill K (of_val v) @ ↑c; E {{Ψ}})
+  (∀ K Ψ, (⚡◻{ Ω ↑ c } ∀ v, Φ v -∗ WP fill K (of_val v) @ ↑c; E {{Ψ}})
             -∗ WP fill K e @ ↑c; E {{Ψ}})%I.
 Definition clwp_aux : seal (@clwp_def). by eexists. Qed.
 Definition clwp := unseal clwp_aux.
@@ -51,14 +51,14 @@ Section clwp.
   
   Lemma clwp_cl {c E e Φ} K :
     CLWP e @ ↑c; E {{Φ}} -∗
-    (∀ Ψ, (∀ v, Φ v -∗ WP fill K (of_val v) @ ↑c; E {{Ψ}})
+    (∀ Ψ, (⚡◻{ Ω ↑ c } ∀ v, Φ v -∗ WP fill K (of_val v) @ ↑c; E {{Ψ}})
             -∗ WP fill K e @ ↑c; E {{Ψ}})%I.
   Proof. rewrite clwp_eq /clwp_def. iIntros "H". iIntros (?). iApply "H". Qed.
 
   (* Weakest pre *)
   Lemma unfold_clwp (c : C) (E : coPset) (e : expr) (Φ : val → iProp Σ) :
     CLWP e @ ↑c; E {{Φ}} ⊣⊢
-         (∀ K Ψ, (∀ v, Φ v -∗ WP fill K (of_val v) @ ↑c; E {{Ψ}})
+         (∀ K Ψ, (⚡◻{ Ω ↑ c } ∀ v, Φ v -∗ WP fill K (of_val v) @ ↑c; E {{Ψ}})
                    -∗ WP fill K e @ ↑c; E {{Ψ}})%I.
   Proof. by rewrite clwp_eq /clwp_def. Qed.
 
@@ -67,7 +67,8 @@ Section clwp.
   Proof.
     iIntros "H". rewrite unfold_clwp.
     iSpecialize ("H" $! empty_ectx Φ with "[]").
-    - iIntros (w) "Hw". rewrite -> CC_fill_empty.
+    - iApply bnextgen_ind_from_plainly. iModIntro.
+      iIntros (w) "Hw". rewrite -> CC_fill_empty.
       iApply wp_value; rewrite /IntoVal /=; eauto using to_of_val.
     - by rewrite CC_fill_empty.
   Qed.
@@ -76,7 +77,7 @@ Section clwp.
     Proper (pointwise_relation _ (dist n) ==> dist n) (@clwp _ _ _ _ _ Λ _ Σ _ _ _ c E e).
   Proof.
     repeat intros?; rewrite !unfold_clwp.
-    repeat (repeat apply forall_ne=>?; repeat apply wand_ne; trivial).
+    repeat (repeat apply forall_ne=>?; repeat apply bnextgen_ind_ne; repeat apply wand_ne; trivial).
   Qed.
   Global Instance clwp_proper c E e :
     Proper (pointwise_relation _ (≡) ==> (≡)) (@clwp _ _ _ _ _ Λ _ Σ _ _ _ c E e).
@@ -87,7 +88,7 @@ Section clwp.
   Lemma clwp_value' c E Φ v : Φ v ⊢ CLWP of_val v @ ↑c; E {{ Φ }}.
   Proof.
     iIntros "HΦ"; rewrite unfold_clwp.
-    iIntros (K Ψ) "HK". iApply ("HK" with "HΦ").
+    iIntros (K Ψ) "HK". rewrite bnextgen_bounded_ind_elim. iApply ("HK" with "HΦ").
   Qed.
   Lemma clwp_value_inv c E Φ v : CLWP of_val v @ ↑c; E {{ Φ }} ={E}=∗ Φ v.
   Proof. iIntros "H"; iApply wp_value_fupd'. by iApply clwp_wp. Qed.
@@ -101,7 +102,7 @@ Section clwp.
   Proof.
     iIntros "H"; rewrite !unfold_clwp.
     iIntros (K Ψ) "HK".
-    iApply "H". iIntros (w) ">Hw"; by iApply "HK".
+    iApply "H". iApply (bnextgen_ind_mono with "HK");iIntros "HK". iIntros (w) ">Hw"; by iApply "HK".
   Qed.
 
   Lemma clwp_bind c K E e Φ :
@@ -110,9 +111,14 @@ Section clwp.
   Proof.
     iIntros "H"; rewrite !unfold_clwp. iIntros (K' Ψ) "HK'".
     rewrite CC_fill_comp.
-    iApply "H"; iIntros (v) "Hv".
+    iApply "H".
+    rewrite bnextgen_bounded_ind_idemp.
+    iApply (bnextgen_ind_mono with "HK'");iIntros "HK'".
+    iIntros (v) "Hv".
     rewrite !unfold_clwp -CC_fill_comp.
-    iApply "Hv"; iIntros (w) "Hw".
+    iApply "Hv".
+    iApply (bnextgen_ind_mono with "HK'");iIntros "HK'".
+    iIntros (w) "Hw".
     by iApply "HK'".
   Qed.
 
@@ -121,7 +127,9 @@ Section clwp.
     CLWP e @ ↑c; E {{ Φ }} ⊢ CLWP e @ ↑c; E {{ Ψ }}.
   Proof.
     iIntros (HΦ) "H"; rewrite !unfold_clwp. iIntros (K χ) "HK".
-    iApply "H". iIntros (w) "Hw". iApply "HK"; by iApply HΦ.
+    iApply "H".
+    iApply (bnextgen_ind_mono with "HK");iIntros "HK".
+    iIntros (w) "Hw". iApply "HK"; by iApply HΦ.
   Qed.
   Global Instance clwp_mono' c E e :
     Proper (pointwise_relation _ (⊢) ==> (⊢)) (@clwp _ _ _ _ _ Λ _ Σ _ _ _ c E e).
@@ -137,30 +145,39 @@ Section clwp.
   Proof. intros. rewrite -clwp_fupd -clwp_value //. Qed.
 
   Lemma clwp_frame_l c E e Φ R :
-    R ∗ CLWP e @ ↑c; E {{ Φ }} ⊢ CLWP e @ ↑c; E {{ v, R ∗ Φ v }}.
+    (⚡◻{ Ω ↑ c } R) ∗ CLWP e @ ↑c; E {{ Φ }} ⊢ CLWP e @ ↑c; E {{ v, R ∗ Φ v }}.
   Proof.
     iIntros "[HR H]"; rewrite !unfold_clwp. iIntros (K Ψ) "HK".
-    iApply "H". iIntros (v) "Hv". iApply "HK"; iFrame.
+    iApply "H".
+    iDestruct (bnextgen_ind_sep with "[$HR $HK]") as "HR".
+    iApply (bnextgen_ind_mono with "HR");iIntros "[HR HK]".
+    iIntros (v) "Hv". iApply "HK"; iFrame.
   Qed.
   Lemma clwp_frame_r c E e Φ R :
-    CLWP e @ ↑c; E {{ Φ }} ∗ R ⊢ CLWP e @ ↑c; E {{ v, Φ v ∗ R }}.
+    CLWP e @ ↑c; E {{ Φ }} ∗ (⚡◻{ Ω ↑ c } R) ⊢ CLWP e @ ↑c; E {{ v, Φ v ∗ R }}.
   Proof.
     iIntros "[H HR]"; rewrite !unfold_clwp. iIntros (K Ψ) "HK".
-    iApply "H". iIntros (v) "Hv". iApply "HK"; iFrame.
+    iApply "H".
+    iDestruct (bnextgen_ind_sep with "[$HR $HK]") as "HR".
+    iApply (bnextgen_ind_mono with "HR");iIntros "[HR HK]".
+    iIntros (v) "Hv". iApply "HK"; iFrame.
   Qed.
 
   Lemma clwp_wand c E e Φ Ψ :
-    CLWP e @ ↑c; E {{ Φ }} -∗ (∀ v, Φ v -∗ Ψ v) -∗ CLWP e @ ↑c; E {{ Ψ }}.
+    CLWP e @ ↑c; E {{ Φ }} -∗ (⚡◻{ Ω ↑ c } (∀ v, Φ v -∗ Ψ v)) -∗ CLWP e @ ↑c; E {{ Ψ }}.
   Proof.
     iIntros "Hwp H". rewrite !unfold_clwp.
     iIntros (K χ) "HK".
-    iApply "Hwp". iIntros (?) "?"; iApply "HK"; by iApply "H".
+    iApply "Hwp".
+    iDestruct (bnextgen_ind_sep with "[$H $HK]") as "H".
+    iApply (bnextgen_ind_mono with "H");iIntros "[H HK]".    
+    iIntros (?) "?"; iApply "HK"; by iApply "H".
   Qed.
   Lemma clwp_wand_l c E e Φ Ψ :
-    (∀ v, Φ v -∗ Ψ v) ∗ CLWP e @ ↑c; E {{ Φ }} ⊢ CLWP e @ ↑c; E {{ Ψ }}.
+    (⚡◻{ Ω ↑ c } ∀ v, Φ v -∗ Ψ v) ∗ CLWP e @ ↑c; E {{ Φ }} ⊢ CLWP e @ ↑c; E {{ Ψ }}.
   Proof. iIntros "[H Hwp]". iApply (clwp_wand with "Hwp H"). Qed.
   Lemma clwp_wand_r c E e Φ Ψ :
-    CLWP e @ ↑c; E {{ Φ }} ∗ (∀ v, Φ v -∗ Ψ v) ⊢ CLWP e @ ↑c; E {{ Ψ }}.
+    CLWP e @ ↑c; E {{ Φ }} ∗ (⚡◻{ Ω ↑ c } ∀ v, Φ v -∗ Ψ v) ⊢ CLWP e @ ↑c; E {{ Ψ }}.
   Proof. iIntros "[Hwp H]". iApply (clwp_wand with "Hwp H"). Qed.
 End clwp.
 
@@ -173,8 +190,8 @@ Section proofmode_classes.
 
   Global Instance frame_clwp p c E e R Φ Ψ :
     (∀ v, Frame p R (Φ v) (Ψ v)) →
-    Frame p R (CLWP e @ ↑c; E {{ Φ }}) (CLWP e @ ↑c; E {{ Ψ }}).
-  Proof. rewrite /Frame=> HR. rewrite clwp_frame_l. apply clwp_mono, HR. Qed.
+    Frame p (⚡◻{ Ω ↑ c } R) (CLWP e @ ↑c; E {{ Φ }}) (CLWP e @ ↑c; E {{ Ψ }}).
+  Proof. rewrite /Frame=> HR. rewrite bnextgen_bounded_ind_if_always. rewrite clwp_frame_l. apply clwp_mono, HR. Qed.
 
   Global Instance is_except_0_clwp c E e Φ : IsExcept0 (CLWP e @ ↑c; E {{ Φ }}).
   Proof. by rewrite /IsExcept0 -{2}fupd_clwp -except_0_fupd -fupd_intro. Qed.
